Introduce configurations to get ett and ptt from tt.

formalization/tt.v
@@ -1,11 +1,22 @@
-(* The source type theory. *)
-
-Require tt.
-Include tt.economy.
-
-(* OLD STUFF BELOW
+(* Confgurable type theory. *)
 
 Require Import syntax.
+
+Module Type Configuration.
+  Parameter Paranoia : Type.
+End Configuration.
+
+Module Make(C : Configuration).
+
+(* Notations for writing down inference rules. *)
+
+Notation "'rule' r 'endrule'" := (r) (at level 96, only parsing).
+Notation "'parameters:'  x .. y , p" :=
+  ((forall x , .. (forall y , p) ..))
+    (at level 200, x binder, y binder, right associativity, only parsing).
+Notation "'premise:' p q" := (p -> q) (only parsing, at level 95).
+Notation "'precond:' p q" := ((C.Paranoia -> p) -> q) (only parsing, at level 95).
+Notation "'conclusion:' q" := q (no associativity, only parsing, at level 94).
 
 Inductive isctx : context -> Type :=
 
@@ -17,24 +28,31 @@ Inductive isctx : context -> Type :=
      | CtxExtend :
        rule
          parameters: {G A},
+         precond: isctx G
          premise: istype G A
          conclusion: isctx (ctxextend G A)
        endrule
 
+
 with issubst : substitution -> context -> context -> Type :=
 
      | SubstZero :
-       rule
-         parameters: {G u A},
-         premise: isterm G u A
-         conclusion: issubst (sbzero A u) G (ctxextend G A)
-       endrule
+         rule
+           parameters: {G u A},
+           premise: isterm G u A
+           precond: istype G A
+           precond: isctx G
+           conclusion:
+             issubst (sbzero A u) G (ctxextend G A)
+         endrule
 
      | SubstWeak :
        rule
          parameters: {G A},
          premise: istype G A
-         conclusion: issubst (sbweak A) (ctxextend G A) G
+         precond: isctx G
+         conclusion:
+           issubst (sbweak A) (ctxextend G A) G
        endrule
 
      | SubstShift :
@@ -42,8 +60,12 @@ with issubst : substitution -> context -> context -> Type :=
          parameters: {G D A sbs},
          premise: issubst sbs G D
          premise: istype D A
+         precond: isctx G
+         precond: isctx D
          conclusion:
-           issubst (sbshift A sbs) (ctxextend G (Subst A sbs)) (ctxextend D A)
+           issubst (sbshift A sbs)
+                   (ctxextend G (Subst A sbs))
+                   (ctxextend D A)
        endrule
 
      | SubstId :
@@ -58,7 +80,11 @@ with issubst : substitution -> context -> context -> Type :=
          parameters: {G D E sbs sbt},
          premise: issubst sbs G D
          premise: issubst sbt D E
-         conclusion: issubst (sbcomp sbt sbs) G E
+         precond: isctx G
+         precond: isctx D
+         precond: isctx E
+         conclusion:
+           issubst (sbcomp sbt sbs) G E
        endrule
 
      | SubstCtxConv :
@@ -67,9 +93,13 @@ with issubst : substitution -> context -> context -> Type :=
          premise: issubst sbs G1 D1
          premise: eqctx G1 G2
          premise: eqctx D1 D2
-         conclusion: issubst sbs G2 D2
+         precond: isctx G1
+         precond: isctx G2
+         precond: isctx D1
+         precond: isctx D2
+         conclusion:
+           issubst sbs G2 D2
        endrule
-
 
 
 with istype : context -> type -> Type :=
@@ -79,7 +109,10 @@ with istype : context -> type -> Type :=
          parameters: {G D A},
          premise: istype G A
          premise: eqctx G D
-         conclusion: istype D A
+         precond: isctx G
+         precond: isctx D
+         conclusion:
+           istype D A
        endrule
 
      | TySubst :
@@ -87,43 +120,55 @@ with istype : context -> type -> Type :=
          parameters: {G D A sbs},
          premise: issubst sbs G D
          premise: istype D A
-         conclusion: istype G (Subst A sbs)
+         precond: isctx G
+         precond: isctx D
+         conclusion:
+           istype G (Subst A sbs)
        endrule
 
      | TyProd :
        rule
          parameters: {G A B},
          premise: istype (ctxextend G A) B
-         conclusion: istype G (Prod A B)
+         precond: istype G A
+         precond: isctx G
+         conclusion:
+           istype G (Prod A B)
        endrule
 
      | TyId :
        rule
          parameters: {G A u v},
+         precond: isctx G
+         precond: istype G A
          premise: isterm G u A
          premise: isterm G v A
-         conclusion: istype G (Id A u v)
+         conclusion:
+           istype G (Id A u v)
        endrule
 
      | TyEmpty :
        rule
          parameters: {G},
          premise: isctx G
-         conclusion: istype G Empty
+         conclusion:
+           istype G Empty
        endrule
 
      | TyUnit :
        rule
          parameters: {G},
          premise: isctx G
-         conclusion: istype G Unit
+         conclusion:
+           istype G Unit
        endrule
 
      | TyBool :
        rule
          parameters: {G},
          premise: isctx G
-         conclusion: istype G Bool
+         conclusion:
+           istype G Bool
        endrule
 
 
@@ -135,7 +180,11 @@ with isterm : context -> term -> type -> Type :=
          parameters: {G A B u},
          premise: isterm G u A
          premise: eqtype G A B
-         conclusion: isterm G u B
+         precond: isctx G
+         precond: istype G A
+         precond: istype G B
+         conclusion:
+           isterm G u B
        endrule
 
      | TermCtxConv :
@@ -143,7 +192,11 @@ with isterm : context -> term -> type -> Type :=
          parameters: {G D A u},
          premise: isterm G u A
          premise: eqctx G D
-         conclusion: isterm D u A
+         precond: isctx G
+         precond: isctx D
+         precond: istype G A
+         conclusion:
+           isterm D u A
        endrule
 
      | TermSubst :
@@ -151,20 +204,27 @@ with isterm : context -> term -> type -> Type :=
          parameters: {G D A u sbs},
          premise: issubst sbs G D
          premise: isterm D u A
-         conclusion: isterm G (subst u sbs) (Subst A sbs)
+         precond: isctx G
+         precond: istype D A
+         precond: isctx D
+         conclusion:
+           isterm G (subst u sbs) (Subst A sbs)
        endrule
 
      | TermVarZero :
        rule
          parameters: {G A},
+         precond: isctx G
          premise: istype G A
-         conclusion: 
+         conclusion:
            isterm (ctxextend G A) (var 0) (Subst A (sbweak A))
        endrule
 
      | TermVarSucc :
        rule
          parameters: {G A B k},
+         precond: isctx G
+         precond: istype G A
          premise: isterm G (var k) A
          premise: istype G B
          conclusion:
@@ -174,13 +234,20 @@ with isterm : context -> term -> type -> Type :=
      | TermAbs :
        rule
          parameters: {G A u B},
+         precond: isctx G
+         precond: istype G A
+         precond: istype (ctxextend G A) B
          premise: isterm (ctxextend G A) u B
-         conclusion: isterm G (lam A B u) (Prod A B)
+         conclusion:
+           isterm G (lam A B u) (Prod A B)
        endrule
 
      | TermApp :
        rule
          parameters: {G A B u v},
+         precond: isctx G
+         precond: istype G A
+         precond: istype (ctxextend G A) B
          premise: isterm G u (Prod A B)
          premise: isterm G v A
          conclusion:
@@ -190,16 +257,20 @@ with isterm : context -> term -> type -> Type :=
      | TermRefl :
        rule
          parameters: {G A u},
+         precond: isctx G
+         precond: istype G A
          premise: isterm G u A
-         conclusion: isterm G (refl A u) (Id A u u)
+         conclusion:
+           isterm G (refl A u) (Id A u u)
        endrule
 
      | TermJ :
        rule
          parameters: {G A C u v w p},
+         precond: isctx G
+         precond: istype G A
          premise: isterm G u A
-         premise:
-           istype
+         premise: istype
              (ctxextend
                 (ctxextend G A)
                 (Id
@@ -210,23 +281,22 @@ with isterm : context -> term -> type -> Type :=
              )
              C
          premise:
-           isterm
-             G
-             w
-             (Subst
-                (Subst
-                   C
-                   (sbshift
-                      (Id
-                         (Subst A (sbweak A))
-                         (subst u (sbweak A))
-                         (var 0)
-                      )
-                      (sbzero A u)
-                   )
-                )
-                (sbzero (Id A u u) (refl A u))
-             )
+           isterm G
+                  w
+                  (Subst
+                     (Subst
+                        C
+                        (sbshift
+                           (Id
+                              (Subst A (sbweak A))
+                              (subst u (sbweak A))
+                              (var 0)
+                           )
+                           (sbzero A u)
+                        )
+                     )
+                     (sbzero (Id A u u) (refl A u))
+                  )
          premise: isterm G v A
          premise: isterm G p (Id A u v)
          conclusion:
@@ -251,101 +321,127 @@ with isterm : context -> term -> type -> Type :=
      | TermExfalso :
        rule
          parameters: {G A u},
+         precond: isctx G
          premise: istype G A
          premise: isterm G u Empty
-         conclusion: isterm G (exfalso A u) A
+         conclusion:
+           isterm G (exfalso A u) A
        endrule
 
      | TermUnit :
        rule
          parameters: {G},
          premise: isctx G
-         conclusion: isterm G unit Unit
+         conclusion:
+           isterm G unit Unit
        endrule
 
      | TermTrue :
        rule
          parameters: {G},
          premise: isctx G
-         conclusion: isterm G true Bool
+         conclusion:
+           isterm G true Bool
        endrule
 
      | TermFalse :
        rule
          parameters: {G},
          premise: isctx G
-         conclusion: isterm G false Bool
+         conclusion:
+           isterm G false Bool
        endrule
 
      | TermCond :
        rule
          parameters: {G C u v w},
+         precond: isctx G
          premise: isterm G u Bool
          premise: istype (ctxextend G Bool) C
          premise: isterm G v (Subst C (sbzero Bool true))
          premise: isterm G w (Subst C (sbzero Bool false))
          conclusion:
-           isterm
-             G
-             (cond C u v w)
-             (Subst C (sbzero Bool u))
+           isterm G
+                  (cond C u v w)
+                  (Subst C (sbzero Bool u))
        endrule
 
 
 
 with eqctx : context -> context -> Type :=
 
+
      | CtxRefl :
        rule
          parameters: {G},
          premise: isctx G
-         conclusion: eqctx G G
+         conclusion:
+           eqctx G G
        endrule
 
      | CtxSym :
        rule
          parameters: {G D},
          premise: eqctx G D
-         conclusion: eqctx D G
+         precond: isctx G
+         precond: isctx D
+         conclusion:
+           eqctx D G
        endrule
 
      | CtxTrans :
        rule
          parameters: {G D E},
+         precond: isctx G
+         precond: isctx D
+         precond: isctx E
          premise: eqctx G D
          premise: eqctx D E
-         conclusion: eqctx G E
+         conclusion:
+           eqctx G E
        endrule
 
      | EqCtxEmpty :
        rule
-         conclusion: eqctx ctxempty ctxempty
+         conclusion:
+           eqctx ctxempty ctxempty
        endrule
 
      | EqCtxExtend :
        rule
          parameters: {G D A B},
+         precond: isctx G
+         precond: isctx D
+         precond: istype G A
+         precond: istype G B
          premise: eqctx G D
          premise: eqtype G A B
-         conclusion: eqctx (ctxextend G A) (ctxextend D B)
+         conclusion:
+           eqctx (ctxextend G A) (ctxextend D B)
        endrule
-
-
 
 with eqsubst : substitution -> substitution -> context -> context -> Type :=
 
      | SubstRefl :
        rule
          parameters: {G D sbs},
+         precond: isctx G
+         precond: isctx D
          premise: issubst sbs G D
-         conclusion: eqsubst sbs sbs G D
+         conclusion:
+           eqsubst sbs sbs G D
        endrule
 
      | SubstSym :
        rule
          parameters: {G D sbs sbt},
          premise: eqsubst sbs sbt G D
-         conclusion: eqsubst sbt sbs G D
+         precond: issubst sbs G D
+         precond: issubst sbt G D
+         precond: isctx G
+         precond: isctx D
+         conclusion:
+           eqsubst sbt sbs G D
        endrule
 
      | SubstTrans :
@@ -353,7 +449,13 @@ with eqsubst : substitution -> substitution -> context -> context -> Type :=
          parameters: {G D sb1 sb2 sb3},
          premise: eqsubst sb1 sb2 G D
          premise: eqsubst sb2 sb3 G D
-         conclusion: eqsubst sb1 sb3 G D
+         precond: issubst sb1 G D
+         precond: issubst sb2 G D
+         precond: issubst sb3 G D
+         precond: isctx G
+         precond: isctx D
+         conclusion:
+           eqsubst sb1 sb3 G D
        endrule
 
      | CongSubstZero :
@@ -361,24 +463,30 @@ with eqsubst : substitution -> substitution -> context -> context -> Type :=
          parameters: {G A1 A2 u1 u2},
          premise: eqtype G A1 A2
          premise: eqterm G u1 u2 A1
+         precond: isctx G
+         precond: istype G A1
+         precond: istype G A2
+         precond: isterm G u1 A1
+         precond: isterm G u2 A1
          conclusion:
-           eqsubst
-             (sbzero A1 u1)
-             (sbzero A2 u2)
-             G
-             (ctxextend G A1)
+           eqsubst (sbzero A1 u1)
+                   (sbzero A2 u2)
+                   G
+                   (ctxextend G A1)
        endrule
 
      | CongSubstWeak :
        rule
          parameters: {G A1 A2},
          premise: eqtype G A1 A2
+         precond: isctx G
+         precond: istype G A1
+         precond: istype G A2
          conclusion:
-           eqsubst
-             (sbweak A1)
-             (sbweak A2)
-             (ctxextend G A1)
-             G
+           eqsubst (sbweak A1)
+                   (sbweak A2)
+                   (ctxextend G A1)
+                   G
        endrule
 
      | CongSubstShift :
@@ -386,12 +494,17 @@ with eqsubst : substitution -> substitution -> context -> context -> Type :=
          parameters: {G D A1 A2 sbs1 sbs2},
          premise: eqsubst sbs1 sbs2 G D
          premise: eqtype D A1 A2
+         precond: isctx G
+         precond: isctx D
+         precond: istype D A1
+         precond: istype D A2
+         precond: issubst sbs1 G D
+         precond: issubst sbs2 G D
          conclusion:
-           eqsubst
-             (sbshift A1 sbs1)
-             (sbshift A2 sbs2)
-             (ctxextend G (Subst A1 sbs1))
-             (ctxextend D A1)
+           eqsubst (sbshift A1 sbs1)
+                   (sbshift A2 sbs2)
+                   (ctxextend G (Subst A1 sbs1))
+                   (ctxextend D A1)
        endrule
 
      | CongSubstComp :
@@ -399,6 +512,13 @@ with eqsubst : substitution -> substitution -> context -> context -> Type :=
          parameters: {G D E sbs1 sbs2 sbt1 sbt2},
          premise: eqsubst sbs1 sbs2 G D
          premise: eqsubst sbt1 sbt2 D E
+         precond: issubst sbs1 G D
+         precond: issubst sbs2 G D
+         precond: issubst sbt1 D E
+         precond: issubst sbt2 D E
+         precond: isctx G
+         precond: isctx D
+         precond: isctx E
          conclusion:
            eqsubst (sbcomp sbt1 sbs1)
                    (sbcomp sbt2 sbs2)
@@ -412,7 +532,14 @@ with eqsubst : substitution -> substitution -> context -> context -> Type :=
          premise: eqsubst sbs sbt G1 D1
          premise: eqctx G1 G2
          premise: eqctx D1 D2
-         conclusion: eqsubst sbs sbt G2 D2
+         precond: isctx G1
+         precond: isctx G2
+         precond: isctx D1
+         precond: isctx D2
+         precond: issubst sbs G1 D1
+         precond: issubst sbt G1 D1
+         conclusion:
+           eqsubst sbs sbt G2 D2
        endrule
 
      | CompAssoc :
@@ -421,81 +548,98 @@ with eqsubst : substitution -> substitution -> context -> context -> Type :=
          premise: issubst sbs G D
          premise: issubst sbt D E
          premise: issubst sbr E F
+         precond: isctx G
+         precond: isctx D
+         precond: isctx E
+         precond: isctx F
          conclusion:
-           eqsubst
-             (sbcomp sbr (sbcomp sbt sbs))
-             (sbcomp (sbcomp sbr sbt) sbs)
-             G
-             F
+           eqsubst (sbcomp sbr (sbcomp sbt sbs))
+                   (sbcomp (sbcomp sbr sbt) sbs)
+                   G
+                   F
        endrule
 
      | WeakNat :
        rule
          parameters: {G D A sbs},
+         precond: isctx G
+         precond: isctx D
          premise: issubst sbs G D
          premise: istype D A
          conclusion:
-           eqsubst
-             (sbcomp (sbweak A) (sbshift A sbs))
-             (sbcomp sbs (sbweak (Subst A sbs)))
-             (ctxextend G (Subst A sbs))
-             D
+           eqsubst (sbcomp (sbweak A)
+                           (sbshift A sbs))
+                   (sbcomp sbs
+                           (sbweak (Subst A sbs)))
+                   (ctxextend G (Subst A sbs))
+                   D
        endrule
 
      | WeakZero :
        rule
          parameters: {G A u},
+         precond: isctx G
+         precond: istype G A
          premise: isterm G u A
          conclusion:
-           eqsubst
-             (sbcomp (sbweak A) (sbzero A u))
-             sbid
-             G
-             G
+           eqsubst (sbcomp (sbweak A) (sbzero A u))
+                   sbid
+                   G
+                   G
        endrule
 
      | ShiftZero :
        rule
          parameters: {G D A u sbs},
+         precond: isctx G
+         precond: isctx D
+         precond: istype D A
          premise: issubst sbs G D
          premise: isterm D u A
          conclusion:
-           eqsubst
-             (sbcomp (sbshift A sbs)
-                     (sbzero (Subst A sbs) (subst u sbs)))
-             (sbcomp (sbzero A u)
-                     sbs)
-             G
-             (ctxextend D A)
+           eqsubst (sbcomp (sbshift A sbs)
+                           (sbzero (Subst A sbs) (subst u sbs)))
+                   (sbcomp (sbzero A u)
+                           sbs)
+                   G
+                   (ctxextend D A)
        endrule
 
      | CompShift :
        rule
          parameters: {G D E A sbs sbt},
+         precond: isctx G
+         precond: isctx D
+         precond: isctx E
          premise: issubst sbs G D
          premise: issubst sbt D E
          premise: istype E A
          conclusion:
-           eqsubst
-             (sbcomp (sbshift A sbt)
-                     (sbshift (Subst A sbt) sbs))
-             (sbshift A (sbcomp sbt sbs))
-             (ctxextend G (Subst A (sbcomp sbt sbs)))
-             (ctxextend E A)
+           eqsubst (sbcomp (sbshift A sbt)
+                           (sbshift (Subst A sbt) sbs))
+                   (sbshift A (sbcomp sbt sbs))
+                   (ctxextend G (Subst A (sbcomp sbt sbs)))
+                   (ctxextend E A)
        endrule
 
      | CompIdRight :
        rule
          parameters: {G D sbs},
+         precond: isctx G
+         precond: isctx D
          premise: issubst sbs G D
-         conclusion: eqsubst (sbcomp sbs sbid) sbs G D
+         conclusion:
+           eqsubst (sbcomp sbs sbid) sbs G D
        endrule
 
      | CompIdLeft :
        rule
          parameters: {G D sbs},
+         precond: isctx G
+         precond: isctx D
          premise: issubst sbs G D
-         conclusion: eqsubst (sbcomp sbid sbs) sbs G D
+         conclusion:
+           eqsubst (sbcomp sbid sbs) sbs G D
        endrule
 
 
@@ -506,21 +650,32 @@ with eqtype : context -> type -> type -> Type :=
          parameters: {G D A B},
          premise: eqtype G A B
          premise: eqctx G D
-         conclusion: eqtype D A B
+         precond: istype G A
+         precond: istype G B
+         precond: isctx G
+         precond: isctx D
+         conclusion:
+           eqtype D A B
        endrule
 
      | EqTyRefl:
        rule
          parameters: {G A},
+         precond: isctx G
          premise: istype G A
-         conclusion: eqtype G A A
+         conclusion:
+           eqtype G A A
        endrule
 
      | EqTySym :
        rule
          parameters: {G A B},
          premise: eqtype G A B
-         conclusion: eqtype G B A
+         precond: istype G A
+         precond: istype G B
+         precond: isctx G
+         conclusion:
+           eqtype G B A
        endrule
 
      | EqTyTrans :
@@ -528,18 +683,23 @@ with eqtype : context -> type -> type -> Type :=
          parameters: {G A B C},
          premise: eqtype G A B
          premise: eqtype G B C
-         conclusion: eqtype G A C
+         precond: isctx G
+         precond: istype G A
+         precond: istype G B
+         precond: istype G C
+         conclusion:
+           eqtype G A C
        endrule
 
      | EqTyIdSubst :
        rule
          parameters: {G A},
+         precond: isctx G
          premise: istype G A
          conclusion:
-           eqtype
-             G
-             (Subst A sbid)
-             A
+           eqtype G
+                  (Subst A sbid)
+                  A
        endrule
 
      | EqTySubstComp :
@@ -548,96 +708,121 @@ with eqtype : context -> type -> type -> Type :=
          premise: istype E A
          premise: issubst sbs G D
          premise: issubst sbt D E
+         precond: isctx G
+         precond: isctx D
+         precond: isctx E
          conclusion:
-           eqtype
-             G
-             (Subst (Subst A sbt) sbs)
-             (Subst A (sbcomp sbt sbs))
+           eqtype G
+                  (Subst (Subst A sbt) sbs)
+                  (Subst A (sbcomp sbt sbs))
        endrule
+
 
      | EqTySubstProd :
        rule
          parameters: {G D A B sbs},
          premise: issubst sbs G D
-         premise: istype D A
+         precond: istype D A
          premise: istype (ctxextend D A) B
+         precond: isctx G
+         precond: isctx D
          conclusion:
-           eqtype
-             G
-             (Subst (Prod A B) sbs)
-             (Prod (Subst A sbs) (Subst B (sbshift A sbs)))
+           eqtype G
+                  (Subst (Prod A B) sbs)
+                  (Prod (Subst A sbs) (Subst B (sbshift A sbs)))
        endrule
 
      | EqTySubstId :
        rule
          parameters: {G D A u v sbs},
          premise: issubst sbs G D
+         precond: istype D A
          premise: isterm D u A
          premise: isterm D v A
+         precond: isctx G
+         precond: isctx D
          conclusion:
-            eqtype
-              G
-              (Subst (Id A u v) sbs)
-              (Id (Subst A sbs) (subst u sbs) (subst v sbs))
+           eqtype G
+                  (Subst (Id A u v) sbs)
+                  (Id (Subst A sbs) (subst u sbs) (subst v sbs))
        endrule
 
      | EqTySubstEmpty :
        rule
          parameters: {G D sbs},
          premise: issubst sbs G D
+         precond: isctx G
+         precond: isctx D
          conclusion:
-           eqtype
-             G
-             (Subst Empty sbs)
-             Empty
+           eqtype G
+                  (Subst Empty sbs)
+                  Empty
        endrule
 
      | EqTySubstUnit :
        rule
          parameters: {G D sbs},
          premise: issubst sbs G D
+         precond: isctx G
+         precond: isctx D
          conclusion:
-           eqtype
-             G
-             (Subst Unit sbs)
-             Unit
+           eqtype G
+                  (Subst Unit sbs)
+                  Unit
        endrule
 
      | EqTySubstBool :
        rule
          parameters: {G D sbs},
          premise: issubst sbs G D
+         precond: isctx G
+         precond: isctx D
          conclusion:
-           eqtype
-             G
-             (Subst Bool sbs)
-             Bool
+           eqtype G
+                  (Subst Bool sbs)
+                  Bool
        endrule
 
      | EqTyExfalso :
        rule
          parameters: {G A B u},
+         precond: isctx G
          premise: istype G A
          premise: istype G B
          premise: isterm G u Empty
-         conclusion: eqtype G A B
+         conclusion:
+           eqtype G A B
        endrule
 
      | CongProd :
        rule
          parameters: {G A1 A2 B1 B2},
+         precond: isctx G
+         precond: istype G A1
+         precond: istype (ctxextend G A1) A2
+         precond: istype G B1
+         precond: istype (ctxextend G A1) B2
          premise: eqtype G A1 B1
          premise: eqtype (ctxextend G A1) A2 B2
-         conclusion: eqtype G (Prod A1 A2) (Prod B1 B2)
+         conclusion:
+           eqtype G (Prod A1 A2) (Prod B1 B2)
        endrule
 
      | CongId :
        rule
          parameters: {G A B u1 u2 v1 v2},
+         precond: isctx G
+         precond: istype G A
+         precond: istype G B
+         precond: isterm G u1 A
+         precond: isterm G u2 A
+         precond: isterm G v1 A
+         precond: isterm G v2 A
          premise: eqtype G A B
          premise: eqterm G u1 v1 A
          premise: eqterm G u2 v2 A
-         conclusion: eqtype G (Id A u1 u2) (Id B v1 v2)
+         conclusion:
+           eqtype G (Id A u1 u2) (Id B v1 v2)
        endrule
 
      | CongTySubst :
@@ -645,9 +830,15 @@ with eqtype : context -> type -> type -> Type :=
          parameters: {G D A B sbs sbt},
          premise: eqsubst sbs sbt G D
          premise: eqtype D A B
-         conclusion: eqtype G (Subst A sbs) (Subst B sbt)
+         precond: isctx G
+         precond: isctx D
+         precond: istype D A
+         precond: istype D B
+         precond: issubst sbs G D
+         precond: issubst sbt G D
+         conclusion:
+           eqtype G (Subst A sbs) (Subst B sbt)
        endrule
-
 
 
 with eqterm : context -> term -> term -> type -> Type :=
@@ -657,29 +848,49 @@ with eqterm : context -> term -> term -> type -> Type :=
          parameters: {G A B u v},
          premise: eqterm G u v A
          premise: eqtype G A B
-         conclusion: eqterm G u v B
+         precond: isctx G
+         precond: istype G A
+         precond: istype G B
+         precond: isterm G u A
+         precond: isterm G v A
+         conclusion:
+           eqterm G u v B
        endrule
 
      | EqCtxConv :
        rule
          parameters: {G D u v A},
+         precond: isctx G
+         precond: isctx D
+         precond: istype G A
+         precond: isterm G u A
+         precond: isterm G v A
          premise: eqterm G u v A
          premise: eqctx G D
-         conclusion: eqterm D u v A
+         conclusion:
+           eqterm D u v A
        endrule
 
      | EqRefl :
        rule
          parameters: {G A u},
+         precond: isctx G
+         precond: istype G A
          premise: isterm G u A
-         conclusion: eqterm G u u A
+         conclusion:
+           eqterm G u u A
        endrule
 
      | EqSym :
        rule
          parameters: {G A u v},
          premise: eqterm G v u A
-         conclusion: eqterm G u v A
+         precond: isterm G u A
+         precond: isterm G v A
+         precond: istype G A
+         precond: isctx G
+         conclusion:
+           eqterm G u v A
        endrule
 
      | EqTrans :
@@ -687,19 +898,27 @@ with eqterm : context -> term -> term -> type -> Type :=
          parameters: {G A u v w},
          premise: eqterm G u v A
          premise: eqterm G v w A
-         conclusion: eqterm G u w A
+         precond: isctx G
+         precond: istype G A
+         precond: isterm G u A
+         precond: isterm G v A
+         precond: isterm G w A
+         conclusion:
+           eqterm G u w A
        endrule
+
 
      | EqIdSubst :
        rule
          parameters: {G A u},
+         precond: isctx G
+         precond: istype G A
          premise: isterm G u A
          conclusion:
-           eqterm
-             G
-             (subst u sbid)
-             u
-             A
+           eqterm G
+                  (subst u sbid)
+                  u
+                  A
        endrule
 
      | EqSubstComp :
@@ -708,17 +927,22 @@ with eqterm : context -> term -> term -> type -> Type :=
          premise: isterm E u A
          premise: issubst sbs G D
          premise: issubst sbt D E
+         precond: isctx G
+         precond: isctx D
+         precond: isctx E
+         precond: istype E A
          conclusion:
-           eqterm
-             G
-             (subst (subst u sbt) sbs)
-             (subst u (sbcomp sbt sbs))
-             (Subst A (sbcomp sbt sbs))
+           eqterm G
+                  (subst (subst u sbt) sbs)
+                  (subst u (sbcomp sbt sbs))
+                  (Subst A (sbcomp sbt sbs))
        endrule
 
      | EqSubstWeak :
        rule
          parameters: {G A B k},
+         precond: isctx G
+         precond: istype G A
          premise: isterm G (var k) A
          premise: istype G B
          conclusion:
@@ -732,6 +956,8 @@ with eqterm : context -> term -> term -> type -> Type :=
      | EqSubstZeroZero :
        rule
          parameters: {G u A},
+         precond: isctx G
+         precond: istype G A
          premise: isterm G u A
          conclusion:
            eqterm G
@@ -743,6 +969,9 @@ with eqterm : context -> term -> term -> type -> Type :=
      | EqSubstZeroSucc :
        rule
          parameters: {G A B u k},
+         precond: isctx G
+         precond: istype G A
+         precond: istype G B
          premise: isterm G (var k) A
          premise: isterm G u B
          conclusion:
@@ -755,6 +984,8 @@ with eqterm : context -> term -> term -> type -> Type :=
      | EqSubstShiftZero :
        rule
          parameters: {G D A sbs},
+         precond: isctx G
+         precond: isctx D
          premise: issubst sbs G D
          premise: istype D A
          conclusion:
@@ -766,7 +997,10 @@ with eqterm : context -> term -> term -> type -> Type :=
 
      | EqSubstShiftSucc :
        rule
-         parameters: {G D A B sbs k},
+         parameters: { G D A B sbs k },
+         precond: isctx G
+         precond: isctx D
+         precond: istype D B
          premise: issubst sbs G D
          premise: isterm D (var k) B
          premise: istype D A
@@ -780,8 +1014,12 @@ with eqterm : context -> term -> term -> type -> Type :=
      | EqSubstAbs :
        rule
          parameters: {G D A B u sbs},
-         premise: issubst sbs G D
+         precond: isctx G
+         precond: isctx D
+         precond: istype D A
+         precond: istype (ctxextend D A) B
          premise: isterm (ctxextend D A) u B
+         premise: issubst sbs G D
          conclusion:
            eqterm G
                   (subst (lam A B u) sbs)
@@ -797,9 +1035,13 @@ with eqterm : context -> term -> term -> type -> Type :=
      | EqSubstApp :
        rule
          parameters: {G D A B u v sbs},
-         premise: issubst sbs G D
+         precond: isctx G
+         precond: isctx D
+         precond: istype D A
+         precond: istype (ctxextend D A) B
          premise: isterm D u (Prod A B)
          premise: isterm D v A
+         premise: issubst sbs G D
          conclusion:
            eqterm G
                   (subst (app u A B v) sbs)
@@ -816,6 +1058,9 @@ with eqterm : context -> term -> term -> type -> Type :=
          parameters: {G D A u sbs},
          premise: issubst sbs G D
          premise: isterm D u A
+         precond: isctx G
+         precond: isctx D
+         precond: istype D A
          conclusion:
            eqterm G
                   (subst (refl A u) sbs)
@@ -826,6 +1071,9 @@ with eqterm : context -> term -> term -> type -> Type :=
      | EqSubstJ :
        rule
          parameters: {G D A C u v w p sbs},
+         precond: isctx G
+         precond: isctx D
+         precond: istype D A
          premise: issubst sbs G D
          premise: isterm D u A
          premise:
@@ -835,7 +1083,7 @@ with eqterm : context -> term -> term -> type -> Type :=
                 (Id
                    (Subst A (sbweak A))
                    (subst u (sbweak A))
-                   (var 0)
+                 (var 0)
                 )
              )
              C
@@ -897,15 +1145,17 @@ with eqterm : context -> term -> term -> type -> Type :=
                      )
                      sbs
                   )
-         endrule
+       endrule
 
      (* This rule is subsumed by EqTermExfalso *)
      | EqSubstExfalso :
        rule
          parameters: {G D A u sbs},
-         premise: issubst sbs G D
+         precond: isctx G
+         precond: isctx D
          premise: istype D A
          premise: isterm D u Empty
+         premise: issubst sbs G D
          conclusion:
            eqterm G
                   (subst (exfalso A u) sbs)
@@ -916,6 +1166,8 @@ with eqterm : context -> term -> term -> type -> Type :=
      | EqSubstUnit :
        rule
          parameters: {G D sbs},
+         precond: isctx G
+         precond: isctx D
          premise: issubst sbs G D
          conclusion:
            eqterm G
@@ -928,6 +1180,8 @@ with eqterm : context -> term -> term -> type -> Type :=
        rule
          parameters: {G D sbs},
          premise: issubst sbs G D
+         precond: isctx G
+         precond: isctx D
          conclusion:
            eqterm G
                   (subst true sbs)
@@ -939,6 +1193,8 @@ with eqterm : context -> term -> term -> type -> Type :=
        rule
          parameters: {G D sbs},
          premise: issubst sbs G D
+         precond: isctx G
+         precond: isctx D
          conclusion:
            eqterm G
                   (subst false sbs)
@@ -949,9 +1205,11 @@ with eqterm : context -> term -> term -> type -> Type :=
      | EqSubstCond :
        rule
          parameters: {G D C u v w sbs},
+         precond: isctx G
+         precond: isctx D
          premise: issubst sbs G D
          premise: isterm D u Bool
-         premise: istype (ctxextend D Bool) C
+         premise: istype (ctxextend D Bool) C (* TODO: could this be a precond? *)
          premise: isterm D v (Subst C (sbzero Bool true))
          premise: isterm D w (Subst C (sbzero Bool false))
          conclusion:
@@ -967,31 +1225,44 @@ with eqterm : context -> term -> term -> type -> Type :=
      | EqTermExfalso :
        rule
          parameters: {G A u v w},
+         precond: isctx G
+         precond: istype G A
          premise: isterm G u A
          premise: isterm G v A
          premise: isterm G w Empty
-         conclusion: eqterm G u v A
+         conclusion:
+           eqterm G u v A
        endrule
 
      | UnitEta :
        rule
          parameters: {G u v},
+         precond: isctx G
          premise: isterm G u Unit
          premise: isterm G v Unit
-         conclusion: eqterm G u v Unit
+         conclusion:
+           eqterm G u v Unit
        endrule
 
      | EqReflection :
        rule
          parameters: {G A u v w1 w2},
+         precond: isctx G
+         precond: istype G A
+         precond: isterm G u A
+         precond: isterm G v A
          premise: isterm G w1 (Id A u v)
          premise: isterm G w2 (reflective A)
-         conclusion: eqterm G u v A
+         conclusion:
+           eqterm G u v A
        endrule
 
      | ProdBeta :
        rule
          parameters: {G A B u v},
+         precond: isctx G
+         precond: istype G A
+         precond: istype (ctxextend G A) B
          premise: isterm (ctxextend G A) u B
          premise: isterm G v A
          conclusion:
@@ -1004,6 +1275,7 @@ with eqterm : context -> term -> term -> type -> Type :=
      | CondTrue :
        rule
          parameters: {G C v w},
+         precond: isctx G
          premise: istype (ctxextend G Bool) C
          premise: isterm G v (Subst C (sbzero Bool true))
          premise: isterm G w (Subst C (sbzero Bool false))
@@ -1017,6 +1289,7 @@ with eqterm : context -> term -> term -> type -> Type :=
      | CondFalse :
        rule
          parameters: {G C v w},
+         precond: isctx G
          premise: istype (ctxextend G Bool) C
          premise: isterm G v (Subst C (sbzero Bool true))
          premise: isterm G w (Subst C (sbzero Bool false))
@@ -1030,10 +1303,12 @@ with eqterm : context -> term -> term -> type -> Type :=
      | ProdEta :
        rule
          parameters: {G A B u v},
+         precond: isctx G
+         precond: istype G A
+         precond: istype (ctxextend G A) B
          premise: isterm G u (Prod A B)
          premise: isterm G v (Prod A B)
-         premise:
-           eqterm (ctxextend G A)
+         premise: eqterm (ctxextend G A)
                   (app (subst u (sbweak A))
                        (Subst A (sbweak A))
                        (Subst B (sbshift A (sbweak A)))
@@ -1043,15 +1318,17 @@ with eqterm : context -> term -> term -> type -> Type :=
                        (Subst B (sbshift A (sbweak A)))
                        (var 0))
                   B
-         conclusion: eqterm G u v (Prod A B)
+         conclusion:
+           eqterm G u v (Prod A B)
        endrule
 
      | JRefl :
        rule
          parameters: {G A C u w},
+         precond: isctx G
+         precond: istype G A
          premise: isterm G u A
-         premise:
-           istype
+         premise: istype
              (ctxextend
                 (ctxextend G A)
                 (Id
@@ -1060,9 +1337,8 @@ with eqterm : context -> term -> term -> type -> Type :=
                    (var 0)
                 )
              )
-           C
-         premise:
-           isterm G
+             C
+         premise: isterm G
                   w
                   (Subst
                      (Subst
@@ -1101,6 +1377,13 @@ with eqterm : context -> term -> term -> type -> Type :=
      | CongAbs :
        rule
          parameters: {G A1 A2 B1 B2 u1 u2},
+         precond: isctx G
+         precond: istype G A1
+         precond: istype G B1
+         precond: istype (ctxextend G A1) A2
+         precond: istype (ctxextend G A1) B2
+         precond: isterm (ctxextend G A1) u1 A2
+         precond: isterm (ctxextend G A1) u2 A2
          premise: eqtype G A1 B1
          premise: eqtype (ctxextend G A1) A2 B2
          premise: eqterm (ctxextend G A1) u1 u2 A2
@@ -1114,6 +1397,15 @@ with eqterm : context -> term -> term -> type -> Type :=
      | CongApp :
        rule
          parameters: {G A1 A2 B1 B2 u1 u2 v1 v2},
+         precond: isctx G
+         precond: istype G A1
+         precond: istype (ctxextend G A1) A2
+         precond: istype G B1
+         precond: istype (ctxextend G A1) B2
+         precond: isterm G u1 (Prod A1 A2)
+         precond: isterm G v1 (Prod A1 A2)
+         precond: isterm G u2 A1
+         precond: isterm G v2 A1
          premise: eqtype G A1 B1
          premise: eqtype (ctxextend G A1) A2 B2
          premise: eqterm G u1 v1 (Prod A1 A2)
@@ -1128,6 +1420,11 @@ with eqterm : context -> term -> term -> type -> Type :=
      | CongRefl :
        rule
          parameters: {G u1 u2 A1 A2},
+         precond: isctx G
+         precond: istype G A1
+         precond: istype G A2
+         precond: isterm G u1 A1
+         precond: isterm G u2 A1
          premise: eqterm G u1 u2 A1
          premise: eqtype G A1 A2
          conclusion:
@@ -1140,6 +1437,37 @@ with eqterm : context -> term -> term -> type -> Type :=
      | CongJ :
        rule
          parameters: {G A1 A2 C1 C2 u1 u2 v1 v2 w1 w2 p1 p2},
+         precond: isctx G
+         precond: istype G A1
+         precond: istype G A2
+         precond:
+           istype
+             (ctxextend
+                (ctxextend G A1)
+                (Id
+                   (Subst A1 (sbweak A1))
+                   (subst u1 (sbweak A1))
+                   (var 0)
+                )
+             )
+             C1
+         precond:
+           istype
+             (ctxextend
+                (ctxextend G A1)
+                (Id
+                   (Subst A1 (sbweak A1))
+                   (subst u1 (sbweak A1))
+                   (var 0)
+                )
+             )
+             C2
+         precond: isterm G u1 A1
+         precond: isterm G u2 A1
+         precond: isterm G v1 A1
+         precond: isterm G v2 A1
+         precond: isterm G p1 (Id A1 u1 v1)
+         precond: isterm G p2 (Id A1 u1 v1)
          premise: eqtype G A1 A2
          premise: eqterm G u1 u2 A1
          premise:
@@ -1154,8 +1482,42 @@ with eqterm : context -> term -> term -> type -> Type :=
              )
              C1
              C2
+         precond:
+            isterm G
+                  w1
+                  (Subst
+                     (Subst
+                        C1
+                        (sbshift
+                           (Id
+                              (Subst A1 (sbweak A1))
+                              (subst u1 (sbweak A1))
+                              (var 0)
+                           )
+                           (sbzero A1 u1)
+                        )
+                     )
+                     (sbzero (Id A1 u1 u1) (refl A1 u1))
+                  )
+         precond:
+            isterm G
+                  w2
+                  (Subst
+                     (Subst
+                        C1
+                        (sbshift
+                           (Id
+                              (Subst A1 (sbweak A1))
+                              (subst u1 (sbweak A1))
+                              (var 0)
+                           )
+                           (sbzero A1 u1)
+                        )
+                     )
+                     (sbzero (Id A1 u1 u1) (refl A1 u1))
+                  )
          premise:
-           eqterm G
+            eqterm G
                   w1
                   w2
                   (Subst
@@ -1207,6 +1569,15 @@ with eqterm : context -> term -> term -> type -> Type :=
      | CongCond :
        rule
          parameters: {G C1 C2 u1 u2 v1 v2 w1 w2},
+         precond: isctx G
+         precond: istype (ctxextend G Bool) C1
+         precond: istype (ctxextend G Bool) C2
+         precond: isterm G u1 Bool
+         precond: isterm G u2 Bool
+         precond: isterm G v1 (Subst C1 (sbzero Bool true))
+         precond: isterm G v2 (Subst C1 (sbzero Bool true))
+         precond: isterm G w1 (Subst C1 (sbzero Bool false))
+         precond: isterm G w2 (Subst C1 (sbzero Bool false))
          premise: eqterm G u1 u2 Bool
          premise: eqtype (ctxextend G Bool) C1 C2
          premise: eqterm G v1 v2 (Subst C1 (sbzero Bool true))
@@ -1223,6 +1594,13 @@ with eqterm : context -> term -> term -> type -> Type :=
          parameters: {G D A u1 u2 sbs sbt},
          premise: eqsubst sbs sbt G D
          premise: eqterm D u1 u2 A
+         precond: isctx G
+         precond: isctx D
+         precond: istype D A
+         precond: isterm D u1 A
+         precond: isterm D u2 A
+         precond: issubst sbs G D
+         precond: issubst sbt G D
          conclusion:
            eqterm G
                   (subst u1 sbs)
@@ -1230,4 +1608,18 @@ with eqterm : context -> term -> term -> type -> Type :=
                   (Subst A sbs)
        endrule.
 
- END OF OLD STUFF *)
+End Make.
+
+Module ParanoidConfiguration <: Configuration.
+  Inductive ParanoidUnit : Type := paranoia.
+  Definition Paranoia := ParanoidUnit.
+End ParanoidConfiguration.
+
+Module paranoia := Make(ParanoidConfiguration).
+
+Module EconomicConfiguration <: Configuration.
+  Inductive EconomicEmpty : Type :=.
+  Definition Paranoia := EconomicEmpty.
+End EconomicConfiguration.
+
+Module economy := Make(EconomicConfiguration).
