formalization/config_tactics.v
@@ -1,0 +1,29 @@
+Require Import tt.
+
+(* Deal with configuration. *)
+Ltac doConfig :=
+  (* configure the hypotheses *)
+  repeat
+  (match goal with
+   | H : ParanoidConfiguration.Paranoia -> ?A |- _ =>
+     apply (fun (f : ParanoidConfiguration.Paranoia -> A) => f ParanoidConfiguration.paranoia) in H
+   | H : EconomicConfiguration.Paranoia -> _ |- _ =>
+     clear H
+   end) ;
+  (* configure the goal *)
+  match goal with
+  | |- (ParanoidConfiguration.Paranoia -> _) =>
+    (intros _)
+  | |- (EconomicConfiguration.Paranoia -> _) =>
+    let H := fresh "Eco" in
+    (intros H ; now elim H)
+  | _ => idtac
+  end.
+
+(* Perform a tactic and deal with a configuration. *)
+Tactic Notation (at level 0) "config" tactic(t) := doConfig ; t ; doConfig.
+
+Tactic Notation (at level 5) "capply" uconstr(H) := doConfig ; apply H ; doConfig.
+
+Tactic Notation (at level 5) "ceapply" uconstr(H) := doConfig ; eapply H ; doConfig.
+
